.

theories/Data/ITree.v
@@ -16,10 +16,10 @@ Variant itreeF (itree : Type@{U_discourse}) (E : Type@{U_discourse} -> Type@{U_d
 
 #[projections(primitive)]
 CoInductive itree (E : Type@{U_discourse} -> Type@{U_discourse}) (R : Type@{U_discourse}) : Type@{U_discourse} :=
-  go { observe : itreeF (itree E R) E R }.
+  go { observe : itreeF (itree E R) E R } as t.
 
 #[global] Arguments go {E}%_type_scope {R}%_type_scope observe.
-#[global] Arguments observe {E}%_type_scope {R}%_type_scope.
+#[global] Arguments observe {E}%_type_scope {R}%_type_scope t.
 
 Bind Scope itree_scope with itree.
 Delimit Scope itree_scope with itree.
@@ -28,11 +28,13 @@ Notation Ret r := (go (RetF r)).
 Notation Tau t := (go (TauF t)).
 Notation Vis X e k := (go (VisF X e k)).
 
+#[universes(template)]
 Inductive callE {I : Type} {R : Type} : Type -> Type :=
   | Call : I -> callE R.
 
 #[global] Arguments callE : clear implicits.
 
+#[universes(template)]
 Inductive stateE {S : Type} : Type -> Type :=
   | GetS : stateE S
   | PutS : S -> stateE unit.
@@ -41,7 +43,10 @@ Inductive stateE {S : Type} : Type -> Type :=
 
 Section ITREE_METHOD.
 
-Context {E : Type -> Type}.
+Context {E : Type@{U_discourse} -> Type@{U_discourse}}.
+
+Definition itree_trigger : E ~~> itree E :=
+  fun X : Type@{U_small} => fun e : E X => Vis X e (fun x : X => Ret x).
 
 Definition itree_guard {R1 : Type} {R2 : Type} (k0 : R1 -> itree E R2) (ot0 : itreeF (itree E R1) E R1) (CIH : itree E R1 -> itree E R2) : itree E R2 :=
   match ot0 with
@@ -51,35 +56,33 @@ Definition itree_guard {R1 : Type} {R2 : Type} (k0 : R1 -> itree E R2) (ot0 : it
   end.
 
 Definition itree_bind' {R1 : Type} {R2 : Type} (k : R1 -> itree E R2) : itree E R1 -> itree E R2 :=
-  cofix bind' (t : itree E R1) : itree E R2 := itree_guard (R1 := R1) (R2 := R2) k (observe t) bind'.
+  cofix bind' (t : itree E R1) : itree E R2 := itree_guard (R1 := R1) (R2 := R2) k t.(observe) bind'.
 
 #[global]
-Instance itree_isMonad : isMonad (itree E) :=
-  { pure {A : Type} (x : A) := Ret x
-  ; bind {A : Type} {B : Type} (m : itree E A) (k : A -> itree E B) := itree_bind' k m
+Instance itree_isMonad : isMonad@{U_discourse U_discourse} (itree E) :=
+  { pure {A : Type@{U_discourse}} (x : A) := Ret x
+  ; bind {A : Type@{U_discourse}} {B : Type@{U_discourse}} (m : itree E A) (k : A -> itree E B) := itree_bind' (R1 := A) (R2 := B) k m
   }.
 
 #[global]
 Instance itree_isMonadIter : isMonadIter (itree E) :=
-  fun I : Type => fun R : Type => fun step : I -> itree E (I + R) =>
-  cofix iter (i : I) : itree E R := itree_isMonad.(bind) (step i) (B.either (fun i' : I => Tau (iter i')) (fun r : R => Ret r)).
+  fun I : Type => fun R : Type => fun step : I -> itree E (I + R)%type =>
+  cofix iter (i : I) : itree E R := bind (isMonad := itree_isMonad) (step i) (B.either (fun i' : I => Tau (iter i')) (fun r : R => Ret r)).
 
-Definition itree_trigger {E : Type -> Type} : E ~~> itree E :=
-  fun R : Type => fun e : E R => Vis R e (fun x : R => Ret x).
+Definition itree_interpret {M : Type -> Type} {M_isMonad : isMonad M} {M_isMonadIter : isMonadIter M} (handler : E ~~> M) : itree E ~~> M :=
+  fun R : Type@{U_discourse} => monad_iter (M := M) (fun t0 : itree E R =>
+    match t0.(observe) with
+    | RetF r => pure (inr r)
+    | TauF t => pure (inl t)
+    | VisF X e k => bind (M := M) (handler X e) (fun x : X => pure (inl (k x)))
+    end
+  ).
 
-Definition callE_handler {E : Type -> Type} {I : Type} {R : Type} (callee : I -> itree E R) : callE I R ~~> itree E :=
-  @callE_rect I R (fun X : Type => fun _ : callE I R X => itree E X) callee.
+Definition callE_handler {I : Type} {R : Type} : forall callee : I -> itree E R, callE I R ~~> itree E :=
+  @callE_rect I R (fun X : Type => fun _ : callE I R X => itree E X).
 
 Definition stateE_handler {S : Type} : stateE S ~~> B.stateT S (itree E) :=
   @stateE_rect S (fun X : Type => fun _ : stateE S X => B.stateT S (itree E) X) get put.
-
-Definition itree_interpret {M : Type -> Type} {M_isMonad : isMonad M} {M_isMonadIter : isMonadIter M} (handler : E ~~> M) : itree E ~~> M :=
-  fun R : Type => monad_iter (M := M) $ fun t0 : itree E R =>
-    match observe t0 with
-    | RetF r => pure (inr r)
-    | TauF t => pure (inl t)
-    | VisF X e k => bind (handler X e) (fun x : X => pure (inl (k x)))
-    end.
 
 End ITREE_METHOD.
 
@@ -119,30 +122,31 @@ Section RECURSION.
 #[local] Notation endo X := (X -> X).
 
 Definition itree_interpret_mrec {E1 : handlerCat.(CAT.ob)} {E2 : handlerCat.(CAT.ob)} (ctx : E1 ~~> itree (E1 +' E2)) : itree (E1 +' E2) ~~> itree E2 :=
-  fun R : Type@{U_small} => monad_iter $ fun t0 : itree (E1 +' E2) R =>
-    match observe t0 with
+  fun R : Type@{U_discourse} => monad_iter (M := itree E2) (fun t0 : itree (E1 +' E2) R =>
+    match t0.(observe) with
     | RetF r => Ret (inr r)
     | TauF t => Ret (inl t)
     | VisF X e k =>
       match e with
-      | B.inl1 e1 => Ret (inl (bind (ctx X e1) k))
+      | B.inl1 e1 => Ret (inl (ctx X e1 >>= k))
       | B.inr1 e2 => Vis X e2 (fun x : X => pure (inl (k x)))
       end
-    end.
+    end
+  ).
 
 Definition itree_mrec {E : handlerCat.(CAT.ob)} {E' : handlerCat.(CAT.ob)} (ctx : E ~~> itree (E +' E')) : E ~~> itree E' :=
-  fun R : Type@{U_small} => fun e : E R => itree_interpret_mrec (E1 := E) (E2 := E') ctx R (ctx R e).
+  fun R : Type@{U_discourse} => fun e : E R => itree_interpret_mrec (E1 := E) (E2 := E') ctx R (ctx R e).
 
 Definition itree_mrec_fix {E : handlerCat.(CAT.ob)} {E' : handlerCat.(CAT.ob)} (ctx : endo (E ~~> itree (E +' E'))) : E ~~> itree E' :=
   itree_mrec (E := E) (E' := E') (ctx handlerCat_hasCoproduct.(CAT.inl)).
 
-Definition itree_rec {E : handlerCat.(CAT.ob)} {I : Type@{U_small}} {R : Type@{U_small}} (body : I -> itree (callE I R +' E) R) (arg : I) : itree E R :=
+Definition itree_rec {E : handlerCat.(CAT.ob)} {I : Type} {R : Type} (body : I -> itree (callE I R +' E) R) (arg : I) : itree E R :=
   itree_mrec (E := callE I R) (E' := E) (callE_handler body) R (Call arg).
 
-Definition itree_call {E : handlerCat.(CAT.ob)} {I : Type@{U_small}} {R : Type@{U_small}} (arg : I) : itree (callE I R +' E) R :=
+Definition itree_call {E : handlerCat.(CAT.ob)} {I : Type} {R : Type} (arg : I) : itree (callE I R +' E) R :=
   handlerCat_hasCoproduct.(CAT.inl) R (Call arg).
 
-Definition itree_rec_fix {E : handlerCat.(CAT.ob)} {I : Type@{U_small}} {R : Type@{U_small}} (body : endo (I -> itree (callE I R +' E) R)) : I -> itree E R :=
+Definition itree_rec_fix {E : handlerCat.(CAT.ob)} {I : Type} {R : Type} (body : endo (I -> itree (callE I R +' E) R)) : I -> itree E R :=
   itree_rec (E := E) (I := I) (R := R) (body itree_call).
 
 End RECURSION.
