theories/Index/Index.v
@@ -1,22 +1,12 @@
-Require Import PnV.Prelude.SfLib.
-Require Import PnV.Prelude.Notations.
-Require Import PnV.Prelude.Prelude.
-Require Import PnV.Prelude.ClassicalFacts.
-Require Import PnV.Prelude.ConstructiveFacts.
-Require Import PnV.Prelude.Quotient.
-Require Import PnV.Math.BooleanAlgebra.
-Require Import PnV.Math.ClassicalDomainTheory.
-Require Import PnV.Math.DomainTheory.
-Require Import PnV.Math.OrderTheory.
-Require Import PnV.Math.ClassicalSetTheory.
-Require Import PnV.Math.SetTheory.
-Require Import PnV.Math.ThN.
+
+Require Import PnV.Control.Category.
+Require Import PnV.Control.Monad.
+
 Require Import PnV.Data.Aczel.
 Require Import PnV.Data.Graph.
 Require Import PnV.Data.ITree.
 Require Import PnV.Data.Vector.
-Require Import PnV.Control.Category.
-Require Import PnV.Control.Monad.
+
 Require Import PnV.Logic.BasicFol.
 Require Import PnV.Logic.BasicFol2.
 Require Import PnV.Logic.ClassicalFol.
@@ -29,12 +19,28 @@ Require Import PnV.Logic.HilbertFol2.
 Require Import PnV.Logic.MuRec.
 Require Import PnV.Logic.PrimRec.
 Require Import PnV.Logic.PropositionalLogic.
+
+Require Import PnV.Math.BooleanAlgebra.
+Require Import PnV.Math.ClassicalDomainTheory.
+Require Import PnV.Math.ClassicalSetTheory.
+Require Import PnV.Math.DomainTheory.
+Require Import PnV.Math.OrderTheory.
+Require Import PnV.Math.SetTheory.
+Require Import PnV.Math.ThN.
+
+Require Import PnV.Prelude.ClassicalFacts.
+Require Import PnV.Prelude.ConstructiveFacts.
+Require Import PnV.Prelude.Notations.
+Require Import PnV.Prelude.Prelude.
+Require Import PnV.Prelude.Quotient.
+Require Import PnV.Prelude.SfLib.
+
 Require Import PnV.System.BasicITreeTh.
 Require Import PnV.System.FolFramework.
 Require Import PnV.System.Lambda1.
 Require Import PnV.System.Lang.
 Require Import PnV.System.LGS.
-Require Import PnV.System.PGS.
 Require Import PnV.System.P.
+Require Import PnV.System.PGS.
 Require Import PnV.System.Regex.
 Require Import PnV.System.STLC.
