theories/Math/OrderTheory.v
@@ -53,7 +53,7 @@ Proof.
   subst x. eapply IH with (y := f (S O)); eauto. exists (fun n : N => f (S n)); eauto.
 Qed.
 
-Lemma nonexistence_of_decr_seq_implies_Acc {classic : forall P : Prop, P \/ ~ P} {DC : forall X : Type, forall step : X -> X -> Prop, forall x0 : X, (forall x, exists x', step x x') -> exists seq : nat -> X, seq O = x0 /\ ⟪ STEP : forall n : nat, step (seq n) (seq (S n)) ⟫} {A : Type} (R : A -> A -> Prop) (x : A)
+Lemma nonaccessibility_implies_existence_of_decr_seq {classic : forall P : Prop, P \/ ~ P} {DC : forall X : Type, forall step : X -> X -> Prop, forall x0 : X, (forall x, exists x', step x x') -> exists seq : nat -> X, seq O = x0 /\ ⟪ STEP : forall n : nat, step (seq n) (seq (S n)) ⟫} {A : Type} (R : A -> A -> Prop) (x : A)
   (NOT_ACC : ~ Acc R x)
   : exists f : nat -> A, f O = x /\ ⟪ DECR : forall n : nat, R (f (S n)) (f n) ⟫.
 Proof.
@@ -70,10 +70,8 @@ Proof.
   set (step := fun x : X => fun x' : X => R (proj1_sig x') (proj1_sig x)).
   assert (STEP : forall x : X, exists x' : X, step x x').
   { intros [a Ha]. pose proof (not_Acc_step a Ha) as [b [Hab Hb]]. exists (@exist _ _ b Hb). exact Hab. }
-  pose proof (DC X step (@exist _ _ x NOT_ACC) STEP) as (g & Hg0 & Hstep); unnw.
-  contradiction NO_SEQ. exists (fun n => proj1_sig (g n)). split.
-  - change (proj1_sig (g 0) = x). now rewrite Hg0.
-  - exact Hstep.
+  pose proof (DC X step (@exist _ _ x NOT_ACC) STEP) as (g & Hg & Hstep); unnw.
+  contradiction NO_SEQ. exists (fun n => proj1_sig (g n)). split; ss. now rewrite Hg.
 Qed.
 
 Lemma well_founded_implies_nonexistence_of_decr_seq {A : Type} (R : A -> A -> Prop)
